rename Big.state to big_state

thys/Real_Time_Deque/Big.thy
@@ -6,13 +6,15 @@ begin
 
 text \<open>\<^noindent> The bigger end of the deque during transformation can be in two phases:
 
- \<^descr> \<open>Reverse\<close>: Using the \<open>step\<close> function the originally contained elements, which will be kept in this end, are reversed.
- \<^descr> \<open>Common\<close>: Specified in theory \<open>Common\<close>. Is used to reverse the elements from the previous phase again to get them in the original order.
+ \<^descr> \<open>Reverse\<close>: Using the \<open>step\<close> function the originally contained elements, 
+    which will be kept in this end, are reversed.
+ \<^descr> \<open>Common\<close>: Specified in theory \<open>Common\<close>. Is used to reverse the elements from the previous phase 
+    again to get them in the original order.
 
 \<^noindent> Each phase contains a \<open>current\<close> state, which holds the original elements of the deque end. 
 \<close>
 
-datatype (plugins del: size) 'a state = 
+datatype (plugins del: size) 'a big_state = 
      Reverse "'a current" "'a stack" "'a list" nat
    | Common "'a Common.state"
 
@@ -21,10 +23,10 @@ text \<open>\<^noindent> Functions:
 \<^descr> \<open>push\<close>, \<open>pop\<close>: Add and remove elements using the \<open>current\<close> state.
 \<^descr> \<open>step\<close>: Executes one step of the transformation\<close>
 
-instantiation state ::(type) step
+instantiation big_state ::(type) step
 begin
 
-fun step_state :: "'a state \<Rightarrow> 'a state" where
+fun step_big_state :: "'a big_state \<Rightarrow> 'a big_state" where
   "step (Common state) = Common (step state)"
 | "step (Reverse current _ aux 0) = Common (normalize (Copy current aux [] 0))"
 | "step (Reverse current big aux count) = 
@@ -33,12 +35,13 @@ fun step_state :: "'a state \<Rightarrow> 'a state" where
 instance..
 end
 
-fun push :: "'a \<Rightarrow> 'a state \<Rightarrow> 'a state" where
+fun push :: "'a \<Rightarrow> 'a big_state \<Rightarrow> 'a big_state" where
   "push x (Common state) = Common (Common.push x state)"
 | "push x (Reverse current big aux count) = Reverse (Current.push x current) big aux count"
 
-fun pop :: "'a state \<Rightarrow> 'a * 'a state" where
+fun pop :: "'a big_state \<Rightarrow> 'a * 'a big_state" where
   "pop (Common state) = (let (x, state) = Common.pop state in (x, Common state))"
-| "pop (Reverse current big aux count) = (first current, Reverse (drop_first current) big aux count)"
+| "pop (Reverse current big aux count) = 
+    (first current, Reverse (drop_first current) big aux count)"
 
 end
