thys/Real_Time_Deque/Big_Aux.thy
@@ -10,21 +10,21 @@ text \<open>\<^noindent> Functions:
 \<^descr> \<open>list\<close>: List abstraction of the elements which this end will contain after the transformation is finished
 \<^descr> \<open>list_current\<close>: List abstraction of the elements currently in this deque end.\<close>
 
-fun list :: "'a state \<Rightarrow> 'a list" where
+fun list :: "'a big_state \<Rightarrow> 'a list" where
   "list (Common common) = Common_Aux.list common"
 | "list (Reverse (Current extra _ _ remained) big aux count) = (
    let reversed = take_rev count (Stack_Aux.list big) @ aux in
     extra @ (take_rev remained reversed)
   )"
 
-fun list_current :: "'a state \<Rightarrow> 'a list" where
+fun list_current :: "'a big_state \<Rightarrow> 'a list" where
   "list_current (Common common) = Common_Aux.list_current common"
 | "list_current (Reverse current _ _ _) = Current_Aux.list current"
 
-instantiation state ::(type) invar
+instantiation big_state ::(type) invar
 begin
 
-fun invar_state :: "'a state \<Rightarrow> bool" where
+fun invar_big_state :: "'a big_state \<Rightarrow> bool" where
   "invar (Common state) \<longleftrightarrow> invar state"
 | "invar (Reverse current big aux count) \<longleftrightarrow> (
    case current of Current extra added old remained \<Rightarrow>
@@ -40,30 +40,30 @@ fun invar_state :: "'a state \<Rightarrow> bool" where
 instance..
 end
 
-instantiation state ::(type) size
+instantiation big_state ::(type) size
 begin
 
-fun size_state :: "'a state \<Rightarrow> nat" where
+fun size_big_state :: "'a big_state \<Rightarrow> nat" where
   "size (Common state) = size state"
 | "size (Reverse current _ _ _) = min (size current) (size_new current)"
 
 instance..
 end
 
-instantiation state ::(type) size_new
+instantiation big_state ::(type) size_new
 begin
 
-fun size_new_state :: "'a state \<Rightarrow> nat" where
+fun size_new_big_state :: "'a big_state \<Rightarrow> nat" where
   "size_new (Common state) = size_new state"
 | "size_new (Reverse current _ _ _) = size_new current"
 
 instance..
 end
 
-instantiation state ::(type) remaining_steps
+instantiation big_state ::(type) remaining_steps
 begin
 
-fun remaining_steps_state :: "'a state \<Rightarrow> nat" where
+fun remaining_steps_big_state :: "'a big_state \<Rightarrow> nat" where
   "remaining_steps (Common state) = remaining_steps state"
 | "remaining_steps (Reverse (Current _ _ _ remaining) _ _ count) = count + remaining + 1"
 
