thys/Real_Time_Deque/RealTimeDeque_Dequeue_Proof.thy
@@ -332,7 +332,7 @@ next
     then obtain small_current small_idle big_current big_idle where idle [simp]: "
       States Left big_stepped small_stepped = 
       States Left 
-          (Big.state.Common (state.Idle big_current big_idle))
+          (big_state.Common (state.Idle big_current big_idle))
           (Small.state.Common (state.Idle small_current small_idle))
       "
       using remaining_steps_idle' invar_stepped remaining_steps_stepped
@@ -420,7 +420,7 @@ next
     then obtain small_current small_idle big_current big_idle where idle [simp]: "
       States Right big_stepped small_stepped = 
       States Right 
-          (Big.state.Common (state.Idle big_current big_idle))
+          (big_state.Common (state.Idle big_current big_idle))
           (Small.state.Common (state.Idle small_current small_idle))
       "
       using remaining_steps_idle' invar_stepped remaining_steps_stepped
